Start reimplementing low-level verifier against intermediate spec

steel/Veritas.SteelSel.Verifier.fsti
@@ -6,450 +6,209 @@ open Steel.SelArray
 open FStar.Ghost
 module U32 = FStar.UInt32
 module U64 = FStar.UInt64
-open Veritas.SteelSel.VCache
-open Veritas.Steel.Types
+// open Veritas.SteelSel.VCache
+// open Veritas.Steel.Types
 
-module MSH = Veritas.MultiSetHashDomain
-let model_hash = erased MSH.mset_ms_hashfn_dom
+module K = Veritas.Key
+module R = Veritas.Record
+module L = Veritas.Intermediate.Logs
+module S = Veritas.Intermediate.Store
+module V = Veritas.Intermediate.Verify
+module VC = Veritas.Intermediate.VerifierConfig
+module MS = Veritas.MultiSetHashDomain
 
-[@@erasable]
-noeq
-type thread_state_model = {
-  model_failed : bool;
-  model_store  : VCache.contents;
-  model_clock  : erased U64.t;
-  model_hadd   : model_hash;
-  model_hevict : model_hash;
-}
+#set-options "--ide_id_info_off"
 
+(** Definition of the low-level thread state datatype **)
+
+// AF: Some assumed types for low-level versions of intermediate types
+val data_key_t: Type0
+val key_v (k:data_key_t) : K.data_key
+val data_value_t: Type0
+val value_v (v:data_value_t) : R.data_value
+
+(* Low-level definition of slot_id *)
+let slot_t (vcfg:VC.verifier_config) = (i:U32.t{U32.v i < VC.store_size vcfg})
+
+// AF: Temporary placeholder for low-level clock.
+// Should be replaced by the appropriate low-level type
+let timestamp_t = ref MS.timestamp
+
+// AF: Placeholder for low-level version of the thread local store
+val vstore_t (vcfg:VC.verifier_config) : Type0
+// AF: This will be implemented as an array.
+// But it also needs to encapsulate the invariants to provide a selector to store
+// instead of store_raw
+// A simple way would be to add those as pure predicates in the slprop, but
+// an easier mechanism for selector invariants/refinements would be useful
+val vstore_sl (#vcfg:_) (st:vstore_t vcfg) : slprop u#1
+val vstore_sel (#vcfg:_) (st:vstore_t vcfg) : selector (S.vstore vcfg) (vstore_sl st)
+[@@__steel_reduce__]
+let is_vstore' #vcfg (st:vstore_t vcfg) : vprop' =
+  { hp = vstore_sl st;
+    t = S.vstore vcfg;
+    sel = vstore_sel st }
+unfold
+let is_vstore #vcfg (st:vstore_t vcfg) : vprop = VUnit (is_vstore' st)
+[@@ __steel_reduce__]
+let v_st (#p:vprop) (#vcfg:_) (st:vstore_t vcfg)
+  (h:rmem p{FStar.Tactics.with_tactic selector_tactic (can_be_split p (is_vstore st) /\ True)})
+  : GTot (S.vstore vcfg)
+  = h (is_vstore st)
+
+val vstore_get_record (#vcfg:_) (st:vstore_t vcfg) (s:slot_t vcfg)
+  : SteelSel
+      (option (S.vstore_entry vcfg))
+      (is_vstore st)
+      (fun _ -> is_vstore st)
+      (requires fun h -> U32.v s < length (v_st st h))
+      (ensures fun h0 res h1 ->
+        // AF: Need to repeat the precondition for now, will be fixed in Steel
+        U32.v s < length (v_st st h0) /\
+        // Framing
+        v_st st h0 == v_st st h1 /\
+        // Functional correctness
+        res == Seq.index (v_st st h1) (U32.v s))
+
+val vstore_update_record (#vcfg:_) (st:vstore_t vcfg) (s:slot_t vcfg) (r:data_value_t)
+  : SteelSel unit
+      (is_vstore st)
+      (fun _ -> is_vstore st)
+      (requires fun h0 -> U32.v s < length (v_st st h0) /\
+        S.inuse_slot (v_st st h0) (U32.v s) /\
+        K.is_data_key (S.stored_key (v_st st h0) (U32.v s)))
+      (ensures fun h0 _ h1 ->
+        // AF: Need to repeat the precondition for now, will be fixed in Steel
+        U32.v s < length (v_st st h0) /\
+        S.inuse_slot (v_st st h0) (U32.v s) /\
+        K.is_data_key (S.stored_key (v_st st h0) (U32.v s)) /\
+        // Functional correctness
+        v_st st h1 == S.update_value (v_st st h0) (U32.v s) (R.DVal (value_v r)))
+
+
+// AF: Placeholder for the low-level version of the multiset hash
 val prf_set_hash : Type0
-
 // AF: Internally, should probably be implemented with a ghost reference to the model_hash
 // The selector would then fetch the value in the ghost state
 // The reason why we would need a ghost state is that the "spec" contains strictly more
 // information than the concrete value. So we cannot reconstruct it out of just the concrete state
 val prf_set_hash_sl (_:prf_set_hash) : slprop u#1
-val prf_set_hash_sel (r:prf_set_hash) : selector (model_hash) (prf_set_hash_sl r)
+val prf_set_hash_sel (r:prf_set_hash) : selector MS.ms_hash_value (prf_set_hash_sl r)
 [@@__steel_reduce__]
 let prf_set_hash_inv' (r:prf_set_hash) : vprop' =
   { hp = prf_set_hash_sl r;
-    t = model_hash;
+    t = MS.ms_hash_value;
     sel = prf_set_hash_sel r}
 unfold
 let prf_set_hash_inv (r:prf_set_hash) : vprop = VUnit (prf_set_hash_inv' r)
 
+(* Standard Steel helper to access the selector of the hash without repeating the slprop *)
 [@@ __steel_reduce__]
 let v_hash (#p:vprop) (r:prf_set_hash)
   (h:rmem p{FStar.Tactics.with_tactic selector_tactic (can_be_split p (prf_set_hash_inv r) /\ True)})
-  : GTot model_hash
+  : GTot MS.ms_hash_value
   = h (prf_set_hash_inv r)
 
-let thread_id = U32.t
-let counter_t = ref U64.t
-
+(* Low-level struct representing the current state of a thread *)
 noeq
-type thread_state_t = {
-  id           : thread_id;
-  st           : vstore;  //a map from keys (cache ids) to merkle leaf or internal nodes
-  clock        : counter_t;
+type thread_state_t vcfg = {
+  failed       : ref bool;
+  id           : L.thread_id;
+  st           : vstore_t vcfg;  //a map from keys (cache ids) to merkle leaf or internal nodes
+  clock        : timestamp_t;
   hadd         : prf_set_hash; //current incremental set hash values; TODO
   hevict       : prf_set_hash;
-  failed       : ref bool
 }
 
+(* The separation logic assertion representing the validity of the thread state *)
 [@@__reduce__; __steel_reduce__]
-let thread_state_inv (t:thread_state_t) : vprop =
+let thread_state_inv #vcfg (t:thread_state_t vcfg) : vprop =
   is_vstore t.st `star`
   vptr t.clock `star`
   vptr t.failed `star`
   prf_set_hash_inv t.hadd `star`
   prf_set_hash_inv t.hevict
 
+
+(* An abstraction on top of the thread selector state to match with the intermediate
+   thread state representation *)
 [@@ __steel_reduce__]
 unfold
-let v_thread (#p:vprop) (t:thread_state_t)
+let v_thread (#p:vprop) (#vcfg:_) (t:thread_state_t vcfg)
   (h:rmem p{FStar.Tactics.with_tactic selector_tactic (can_be_split p (thread_state_inv t) /\ True)})
-  : GTot thread_state_model
-  = {
-      model_failed = sel t.failed (focus_rmem h (thread_state_inv t));
-      model_store = asel t.st (focus_rmem h (thread_state_inv t));
-      model_clock = sel t.clock (focus_rmem h (thread_state_inv t));
-      model_hadd = v_hash t.hadd (focus_rmem h (thread_state_inv t));
-      model_hevict = v_hash t.hevict (focus_rmem h (thread_state_inv t))
-    }
+  : GTot (V.vtls vcfg)
+  = if sel t.failed (focus_rmem h (thread_state_inv t)) then
+      V.Valid
+        t.id
+        (v_st t.st (focus_rmem h (thread_state_inv t)))
+        (sel t.clock (focus_rmem h (thread_state_inv t)))
+        (v_hash t.hadd (focus_rmem h (thread_state_inv t)))
+        (v_hash t.hevict (focus_rmem h (thread_state_inv t)))
+    else V.Failed
 
 
-
-
-let model_fail tsm = {tsm with model_failed = false}
-
-let fail (vs:thread_state_t) (msg:string)
+(* Updates the thread state to a Failed state *)
+let fail #vcfg (vs:thread_state_t vcfg) (msg:string)
+  // AF: We put it in SteelSelF to avoid simplify its use in branches because we currently
+  // cannot have SteelSel and SteelSelF branches at the same time, but it shouldn't be
   : SteelSelF unit
              (thread_state_inv vs)
              (fun _ -> thread_state_inv vs)
              (requires fun _ -> True)
-             (ensures fun h0 _ h1 -> v_thread vs h1 == model_fail (v_thread vs h0))
-  = write vs.failed false; ()
+             (ensures fun _ _ h1 -> v_thread vs h1 == V.Failed)
+  = // AF: Need trailing unit to trigger framing. Will be solved once we have framing subcomp
+    write vs.failed false; ()
 
-let slot (tsm:thread_state_model) = (i:U32.t{U32.v i < length tsm.model_store})
-
-let vget_model (tsm:thread_state_model) (s:slot tsm) (v:value) : thread_state_model =
-  match Seq.index tsm.model_store (U32.v s) with
-  | None -> model_fail tsm
-  | Some r' ->
-    if v = r'.record_value then tsm else model_fail tsm
-
-#push-options "--fuel 0 --ifuel 0"
-
-let vget (s:U32.t) (v:value) (vs: thread_state_t)
+(* An implementation of Veritas.Intermediate.Verify.vget *)
+let vget (#vcfg:_) (s:slot_t vcfg) (k:data_key_t) (v:data_value_t) (vs:thread_state_t vcfg)
   : SteelSel unit
              (thread_state_inv vs)
              (fun _ -> thread_state_inv vs)
-             (requires fun h -> U32.v s < length (v_thread vs h).model_store)
+             (requires fun h0 ->
+               U32.v s < length (v_st vs.st h0) /\
+               V.Valid? (v_thread vs h0))
              (ensures fun h0 _ h1 ->
-               U32.v s < length (v_thread vs h0).model_store /\
-               v_thread vs h1 == vget_model (v_thread vs h0) s v
+               V.Valid? (v_thread vs h0) /\
+               v_thread vs h1 == V.vget (U32.v s) (key_v k) (value_v v) (v_thread vs h0)
              )
-  = // AF: Unclear why this get is needed, already observed in smaller examples (cf linked lists).
-    // Without it, the precondition on the selector of thread_state_inv is not propagated.
-    // To debug
+  = // AF: Still unclear why this is needed
     let h = get () in
-    let ro = VCache.vcache_get_record vs.st s in
-    match ro with
-    | None ->
-      fail vs "Slot not found"
+    assert (V.Valid? (v_thread vs h));
+
+    let r0 = vstore_get_record vs.st s in
+    match r0 with
+    | None -> fail vs "VGet: Empty slot"
     | Some r' ->
-      if v = r'.record_value
-      // AF: Usual problem of SteelSel vs SteelSelF difference between the two branches
-      then (noop (); ())
-      else fail vs "Failed: inconsistent key or value in Get"
+      let k' = S.VStoreE?.k r' in
+      let v' = S.VStoreE?.v r' in
+      if key_v k <> k' then fail vs "VGet: Key mismatch"
+      else if R.to_data_value v' <> value_v v then fail vs "VGet: Value mismatch"
+      // AF: Usual problem of Steel vs SteelSel difference in branches
+      else (noop (); ())
 
-let model_get_record (tsm:thread_state_model) (s:slot tsm)
-  : GTot (option record)
-  = Seq.index tsm.model_store (U32.v s)
 
-let model_put_record (tsm:thread_state_model) (s:slot tsm) (r:record)
-  : thread_state_model
-  = {tsm with model_store=Seq.upd tsm.model_store (U32.v s) (Some r)}
-
-let model_evict_record (tsm:thread_state_model) (s:slot tsm)
-  : thread_state_model
-  = {tsm with model_store=Seq.upd tsm.model_store (U32.v s) None }
-
-let vput_model (tsm:thread_state_model) (s:slot tsm) (v:value)
-  : thread_state_model
-  = match model_get_record tsm s with
-    | None -> model_fail tsm
-    | Some r -> model_put_record tsm s ({r with record_value=v})
-
-(* verifier write operation *)
-let vput (s:U32.t) (v:value) (vs: thread_state_t)
+(* An implementation of Veritas.Intermediate.Verify.vput *)
+let vput (#vcfg:_) (s:slot_t vcfg) (k:data_key_t) (v:data_value_t) (vs:thread_state_t vcfg)
   : SteelSel unit
-    (thread_state_inv vs)
-    (fun _ -> thread_state_inv vs)
-    (requires fun h -> U32.v s < length (v_thread vs h).model_store)
-    (ensures fun h0 _ h1 ->
-      U32.v s < length (v_thread vs h0).model_store /\
-      v_thread vs h1 == vput_model (v_thread vs h0) s v)
-  = let h = get() in
-    let ro = VCache.vcache_get_record vs.st s in
-    match ro with
-    | None ->
-      fail vs "Slot not found"
+             (thread_state_inv vs)
+             (fun _ -> thread_state_inv vs)
+             (requires fun h0 ->
+               U32.v s < length (v_st vs.st h0) /\
+               V.Valid? (v_thread vs h0))
+             (ensures fun h0 _ h1 ->
+               V.Valid? (v_thread vs h0) /\
+               v_thread vs h1 == V.vput (U32.v s) (key_v k) (value_v v) (v_thread vs h0)
+             )
+  = // AF: Still unclear why this is needed
+    let h = get () in
+    assert (V.Valid? (v_thread vs h));
 
-    | Some r ->
-      // AF: Again, the SteelSel vs SteelSelF issue requires the extra unit
-      vcache_update_record vs.st s ({ r with record_value = v });
-      ()
-
-val epoch_of_timestamp (t:timestamp) : U32.t
-
-val mk_mhdom (r:record) (t:timestamp) (thread_id:thread_id) : MSH.ms_hashfn_dom
-
-val model_update_hash (h:model_hash) (r:record) (t:timestamp) (thread_id:thread_id)
-  : model_hash
-
-val prf_update_hash (p:prf_set_hash) (r:record) (t:timestamp) (thread_id:thread_id)
-  : SteelSel unit
-    (prf_set_hash_inv p)
-    (fun _ -> prf_set_hash_inv p)
-    (requires fun _ -> True)
-    (ensures fun h0 _ h1 -> v_hash p h1 == model_update_hash (v_hash p h0) r t thread_id)
-
-let model_update_hadd (tsm:_) (r:record) (t:timestamp) (thread_id:thread_id) =
-  ({tsm with model_hadd = model_update_hash tsm.model_hadd r t thread_id})
-
-let update_hadd (r:record) (t:timestamp) (thread_id:thread_id) (vs:thread_state_t)
-  : SteelSel unit
-    (thread_state_inv vs)
-    (fun _ -> thread_state_inv vs)
-    (requires fun _ -> True)
-    (ensures fun h0 _ h1 ->
-      v_thread vs h1 == model_update_hadd (v_thread vs h0) r t thread_id)
-  = // AF: Same as previously
-    let h0 = get () in
-    prf_update_hash vs.hadd r t thread_id;
-    ()
-
-let model_update_hevict (tsm:_) (r:record) (t:timestamp) (thread_id:thread_id) =
-  ({tsm with model_hevict = model_update_hash tsm.model_hevict r t thread_id})
-
-let update_hevict (r:record) (t:timestamp) (thread_id:thread_id) (vs:thread_state_t)
-  : SteelSel unit
-    (thread_state_inv vs)
-    (fun _ -> thread_state_inv vs)
-    (requires fun _ -> True)
-    (ensures fun h0 _ h1 ->
-      v_thread vs h1 == model_update_hevict (v_thread vs h0) r t thread_id)
-  = // AF: Same problem as previously
-    let h0 = get() in
-    prf_update_hash vs.hevict r t thread_id;
-    ()
-
-open FStar.Integers
-
-let model_update_clock (tsm:thread_state_model) (ts:timestamp)
-  : thread_state_model
-  = if FStar.UInt.fits (U64.v tsm.model_clock + U64.v ts) 64
-    then { tsm with model_clock = tsm.model_clock + ts } //+1
-    else model_fail tsm
-
-// AF: Requires some integers reasoningm, but should be straightforward
-val update_clock (ts:timestamp) (vs:thread_state_t)
-  : SteelSel unit
-    (thread_state_inv vs)
-    (fun _ -> thread_state_inv vs)
-    (requires fun _ -> True)
-    (ensures fun h0 _ h1 -> v_thread vs h1 == model_update_clock (v_thread vs h0) ts)
-
-val is_proper_descendent (k0 k1:key) : bool
-
-let mk_record k v am = { record_key = k; record_value = v; record_add_method = am;
-                         record_l_child_in_store = Vfalse;
-                         record_r_child_in_store = Vfalse }
-
-let vaddb_model (tsm:thread_state_model) (s:slot tsm) (r:record) (t:timestamp) (thread_id:thread_id)
-  : thread_state_model
-  = let e = epoch_of_timestamp t in
-    let { record_key = k;
-          record_value = v } = r in
-    (* check value type consistent with key k *)
-    if not (is_value_of k v) then model_fail tsm
-    else if Some? (model_get_record tsm s) then model_fail tsm
-    else (
-      //TODO: need to check that the key does not exist
-      (* updated h_add *)
-      let tsm = model_update_hadd tsm r t thread_id in
-      (* updated clock *)
-      let tsm = model_update_clock tsm t in
-      (* add record to store *)
-      model_put_record tsm s (mk_record k v BAdd)
-    )
-
-let vaddb (s:U32.t)
-          (r:record)
-          (t:timestamp)
-          (thread_id:thread_id)
-          (vs:thread_state_t)
-  : SteelSel unit
-    (thread_state_inv vs)
-    (fun _ -> thread_state_inv vs)
-    (requires fun h -> U32.v s < length (v_thread vs h).model_store)
-    (ensures fun h0 _ h1 ->
-      U32.v s < length (v_thread vs h0).model_store /\
-      v_thread vs h1 == vaddb_model (v_thread vs h0) s r t thread_id)
-  = let h = get() in
-    assert (U32.v s < length (v_thread vs h).model_store);
-    (* epoch of timestamp of last evict *)
-    let e = epoch_of_timestamp t in
-    let { record_key = k;
-          record_value = v } = r in
-    (* check value type consistent with key k *)
-    if not (is_value_of k v)
-    then (
-      fail vs "vaddm: value is incompatible with key"
-    )
-    else (
-      let ro = VCache.vcache_get_record vs.st s in
-      if Some? ro
-      then (
-        fail vs "vaddm: slot s already exists"
-      )
-      else (
-        prf_update_hash vs.hadd r t thread_id;// vs;
-        update_clock t vs;
-        //this next line is tricky for a couple of reasons
-        // 1. the implicit arg to vcache_update_record is unified with the type of `s` which is indexed
-        //    by the original tsm, not the current one
-        // 2. the refinement type mk_record require `is_value_of k v` does not seem to be provable
-        //    here. despite the check above.
-        VCache.vcache_update_record vs.st s (mk_record k v BAdd)      )
-    )
-
-
-let timestamp_lt (t0 t1:timestamp) = t0 `U64.lt` t1
-
-let vevictb_model (tsm:thread_state_model) (s:slot tsm) (t:timestamp) (thread_id:thread_id)
-  : GTot thread_state_model
-  = let e = epoch_of_timestamp t in
-    let clk = tsm.model_clock in
-    if not (clk `timestamp_lt` t)
-    then model_fail tsm
-    else begin
-      (* check that the vstore contains s *)
-      match model_get_record tsm s with
-      | None -> model_fail tsm
-      | Some r ->
-        (* update the evict hash *)
-        let tsm = model_update_hevict tsm r t thread_id in
-        (* advance clock to t *)
-        let tsm = model_update_clock tsm t in
-        (* evict record *)
-        model_evict_record tsm s
-    end
-
-let vevictb (s:U32.t)
-            (t:timestamp)
-            (vs:thread_state_t)
-  : SteelSel unit
-    (thread_state_inv vs)
-    (fun _ -> thread_state_inv vs)
-    (requires fun h -> U32.v s < length (v_thread vs h).model_store)
-    (ensures  fun h0 _ h1 ->
-      U32.v s < length (v_thread vs h0).model_store /\
-      v_thread vs h1 == vevictb_model (v_thread vs h0) s t vs.id)
-  = let h = get() in
-    assert (U32.v s < length (v_thread vs h).model_store);
-    let clk = read vs.clock in
-    if not (clk `timestamp_lt` t)
-    then (
-      fail vs "Timestamp is old"
-    )
-    else (
-      (* check that the vstore contains s *)
-      let r = VCache.vcache_get_record vs.st s in
-      match r with
-      | None ->
-        fail vs "Slot is empty"
-
-      | Some r ->
-        (* update the evict hash *)
-        prf_update_hash vs.hevict r t vs.id;
-
-        update_clock t vs;
-
-        VCache.vcache_evict_record vs.st s)
-
-
-val has_instore_merkle_desc (tsm:thread_state_model) (s:slot tsm) : bool
-
-val has_instore_merkle_desc_impl (s:U32.t) (vs:thread_state_t)
-  : SteelSel bool
-    (requires thread_state_inv vs)
-    (ensures fun _ -> thread_state_inv vs)
-    (requires fun h -> U32.v s < length (v_thread vs h).model_store)
-    (ensures fun h0 b h1 ->
-      U32.v s < length (v_thread vs h0).model_store /\
-      b == has_instore_merkle_desc (v_thread vs h0) s /\
-      v_thread vs h0 == v_thread vs h1)
-
-val desc_dir (k0:key) (k1:key { k0 `is_proper_descendent` k1 }) : bool
-
-val to_merkle_value (v:value) : option mval_value
-
-val desc_hash_dir (v:mval_value) (d:bool) : descendent_hash
-val hashfn (v:value) : hash_value
-val update_merkle_value (v:mval_value) (d:bool) (k:key) (h:hash_value) (b:bool) : mval_value
-val update_in_store (tsm:thread_state_model) (s:slot tsm) (d:bool) (b:bool) : tsm':thread_state_model{Seq.length tsm.model_store = Seq.length tsm'.model_store}
-
-val update_in_store_impl (s:U32.t) (d:bool) (b:bool) (vs:thread_state_t)
-  : SteelSel unit
-    (thread_state_inv vs)
-    (fun _ -> thread_state_inv vs)
-    (requires fun h -> U32.v s < length (v_thread vs h).model_store)
-    (ensures fun h0 _ h1 ->
-      U32.v s < length (v_thread vs h0).model_store /\
-      v_thread vs h1 == update_in_store (v_thread vs h0) s d b)
-
-#push-options "--ifuel 1"
-
-let vevictbm_model (tsm:thread_state_model)
-                   (s s':slot tsm)
-                   (t:timestamp)
-                   (thread_id:thread_id)
-  : thread_state_model
-  = match model_get_record tsm s, model_get_record tsm s' with
-    | Some r, Some r' ->
-      begin
-      if not (is_proper_descendent r.record_key r'.record_key) then model_fail tsm
-      else if has_instore_merkle_desc tsm s then model_fail tsm
-      else if r.record_add_method <> MAdd then model_fail tsm
-      else let d = desc_dir r.record_key r'.record_key in
-           match to_merkle_value r'.record_value with
-           | None -> model_fail tsm //should be impossible, since r' has a proper descendent
-           | Some v' ->
-             let dh' = desc_hash_dir v' d in
-             match dh' with
-             | Dh_vnone _ ->
-               model_fail tsm
-             | Dh_vsome {dhd_key=k2; dhd_h=h2; evicted_to_blum = b2} ->
-               if (k2 <> r.record_key) `Prims.op_BarBar` (b2 = Vtrue)
-               then model_fail tsm
-               else let tsm = model_put_record tsm s' ({r' with record_value=(V_mval (update_merkle_value v' d r.record_key h2 true))}) in
-                    let tsm = update_in_store tsm s' d false in
-                    vevictb_model tsm s t thread_id
-      end
-    | _ -> model_fail tsm
-
-
-let vevictbm (s s':U32.t) (t:timestamp) (vs:thread_state_t)
-  : SteelSel unit
-    (requires thread_state_inv vs)
-    (ensures fun _ -> thread_state_inv vs)
-    (requires fun h ->
-      U32.v s < length (v_thread vs h).model_store /\
-      U32.v s' < length (v_thread vs h).model_store)
-    (ensures fun h0 _ h1 ->
-      U32.v s < length (v_thread vs h0).model_store /\
-      U32.v s' < length (v_thread vs h0).model_store /\
-      v_thread vs h1 == vevictbm_model (v_thread vs h0) s s' t vs.id)
-  = // AF: Same problem as usual
-    let h = get() in
-    assert (U32.v s < length (v_thread vs h).model_store);
-    assert (U32.v s' < length (v_thread vs h).model_store);
-
-    let r = VCache.vcache_get_record vs.st s in
-    let r' = VCache.vcache_get_record vs.st s' in
-    match r, r' with
-    | Some r, Some r' ->
-      if not (is_proper_descendent r.record_key r'.record_key)
-      then fail vs "Not proper descendant"
-      else if has_instore_merkle_desc_impl s vs
-      then fail vs "Not proper descendant"
-      else if r.record_add_method <> MAdd
-      then fail vs "Not merkle add"
-      else (
-           let d = desc_dir r.record_key r'.record_key in
-           match to_merkle_value r'.record_value with
-           | None ->
-             fail vs "should be impossible, since r' has a proper descendent"
-           | Some v' ->
-             let dh' = desc_hash_dir v' d in
-             match dh' with
-             | Dh_vnone _ ->
-               fail vs "no hash in specified direction"
-
-             | Dh_vsome {dhd_key=k2; dhd_h=h2; evicted_to_blum = b2} ->
-               if (k2 <> r.record_key) `Prims.op_BarBar` (b2 = Vtrue)
-               then (
-                 fail vs "no hash in specified direction"
-               )
-               else (
-                 let r'' = {r' with record_value=V_mval (update_merkle_value v' d r.record_key h2 true)} in
-                 VCache.vcache_update_record vs.st s' r'';
-
-                 update_in_store_impl s' d false vs;
-                 vevictb s t vs
-               ))
-    | _ ->
-      fail vs "Records not found"
+    let r0 = vstore_get_record vs.st s in
+    match r0 with
+    | None -> fail vs "VPut: Empty slot"
+    | Some r' ->
+      let k' = S.VStoreE?.k r' in
+      if key_v k <> k' then fail vs "VPut: Key mismatch"
+      // AF: Need the trailing unit to put the body of the else branch into SteelSelF
+      // which is needed since both branches of an if/then/else currently need the same effect
+      else (vstore_update_record vs.st s v; ())
